vale/code/arch/x64/Vale.X64.QuickCodes.fsti
@@ -333,47 +333,69 @@ let rec regs_match (regs:list reg) (r0:Regs.t) (r1:Regs.t) : Type0 =
 [@va_qattr]
 let all_regs_match (r0:Regs.t) (r1:Regs.t) : Type0
   =
-  let regs = [0; 1; 2; 3; 4; 5; 6; 7; 8; 9; 10; 11; 12; 13; 14; 15] in
+  let regs = [
+      Reg 0 0;
+      Reg 0 1;
+      Reg 0 2;
+      Reg 0 3;
+      Reg 0 4;
+      Reg 0 5;
+      Reg 0 6;
+      Reg 0 7;
+      Reg 0 8;
+      Reg 0 9;
+      Reg 0 10;
+      Reg 0 11;
+      Reg 0 12;
+      Reg 0 13;
+      Reg 0 14;
+      Reg 0 15;
+      Reg 1 0;
+      Reg 1 1;
+      Reg 1 2;
+      Reg 1 3;
+      Reg 1 4;
+      Reg 1 5;
+      Reg 1 6;
+      Reg 1 7;
+      Reg 1 8;
+      Reg 1 9;
+      Reg 1 10;
+      Reg 1 11;
+      Reg 1 12;
+      Reg 1 13;
+      Reg 1 14;
+      Reg 1 15
+    ] in
   regs_match regs r0 r1
 
 [@va_qattr]
-let rec xmms_match (xmms:list xmm) (r0:Xmms.t) (r1:Xmms.t) : Type0 =
-  match xmms with
-  | [] -> True
-  | r::xmms -> Xmms.sel r r0 == Xmms.sel r r1 /\ xmms_match xmms r0 r1
-
-[@va_qattr]
-let all_xmms_match (r0:Xmms.t) (r1:Xmms.t) : Type0
+let state_match (s0:vale_state) (s1:vale_state) : Type0
   =
-  let xmms = [0; 1; 2; 3; 4; 5; 6; 7; 8; 9; 10; 11; 12; 13; 14; 15] in
-  xmms_match xmms r0 r1
-
-let assert_norm_match (p:prop0) : Lemma
-  (requires norm [iota; zeta; simplify; primops; delta_only [`%regs_match; `%all_regs_match; `%xmms_match; `%all_xmms_match]] p)
-  (ensures p)
-  =
-  ()
-
-[@va_qattr]
-let va_state_match (s0:vale_state) (s1:vale_state) : Pure Type0
-  (requires True)
-  (ensures fun b -> b ==> state_eq s0 s1)
-  =
-  assert_norm_match (all_regs_match s0.vs_regs s1.vs_regs ==> Regs.equal s0.vs_regs s1.vs_regs);
-  assert_norm_match (all_xmms_match s0.vs_xmms s1.vs_xmms ==> Xmms.equal s0.vs_xmms s1.vs_xmms);
   s0.vs_ok == s1.vs_ok /\
   all_regs_match s0.vs_regs s1.vs_regs /\
-  all_xmms_match s0.vs_xmms s1.vs_xmms /\
   s0.vs_flags == s1.vs_flags /\
   s0.vs_mem == s1.vs_mem /\
   s0.vs_stack == s1.vs_stack /\
   s0.vs_memTaint == s1.vs_memTaint /\
   s0.vs_stackTaint == s1.vs_stackTaint
 
+val lemma_state_match (s0:vale_state) (s1:vale_state) : Lemma
+  (requires state_match s0 s1)
+  (ensures state_eq s0 s1)
+
+[@va_qattr]
+let va_state_match (s0:vale_state) (s1:vale_state) : Pure Type0
+  (requires True)
+  (ensures fun b -> b ==> state_eq s0 s1)
+  =
+  FStar.Classical.move_requires (lemma_state_match s0) s1;
+  state_match s0 s1
+
 [@va_qattr]
 unfold let wp_sound_code_pre (#a:Type0) (#c:code) (qc:quickCode a c) (s0:vale_state) (k:(s0':vale_state{s0 == s0'}) -> vale_state -> a -> Type0) : Type0 =
-  forall (ok:bool) (regs:Regs.t) (xmms:Xmms.t) (flags:nat64) (mem:mem) (stack:stack) (memTaint:memtaint) (stackTaint:memtaint).
-    let s0' = {vs_ok = ok; vs_regs = regs; vs_xmms = xmms; vs_flags = flags; vs_mem = mem; vs_stack = stack; vs_memTaint = memTaint; vs_stackTaint = stackTaint} in
+  forall (ok:bool) (regs:Regs.t) (flags:nat64) (mem:mem) (stack:stack) (memTaint:memtaint) (stackTaint:memtaint).
+    let s0' = {vs_ok = ok; vs_regs = regs; vs_flags = flags; vs_mem = mem; vs_stack = stack; vs_memTaint = memTaint; vs_stackTaint = stackTaint} in
     s0 == s0' ==> QProc?.wp qc (state_eta s0') (k (state_eta s0'))
 
 unfold let wp_sound_code_post (#a:Type0) (#c:code) (qc:quickCode a c) (s0:vale_state) (k:(s0':vale_state{s0 == s0'}) -> vale_state -> a -> Type0) ((sN:vale_state), (fN:fuel), (gN:a)) : Type0 =
@@ -385,7 +407,6 @@ unfold let normal_steps : list string =
   [
     `%Mkvale_state?.vs_ok;
     `%Mkvale_state?.vs_regs;
-    `%Mkvale_state?.vs_xmms;
     `%Mkvale_state?.vs_flags;
     `%Mkvale_state?.vs_mem;
     `%Mkvale_state?.vs_stack;
